WIP

BBSL/BB.v
@@ -1,7 +1,254 @@
 Require Import QArith.
 Require Import BBSL.Interval.
 
+Open Scope Interval_scope.
 
+(** * Definition of [BB] **)
+
+Definition BB : Type := Interval * Interval.
+
+Declare Scope BB_scope.
+Bind Scope BB_scope with BB.
+Delimit Scope BB_scope with BB.
+Open Scope BB_scope.
+
+Definition projx : BB -> Interval := fst.
+Definition projy : BB -> Interval := snd.
+Definition projxl (a : BB) := lb (projx a).
+Definition projxu (a : BB) := ub (projx a).
+Definition projyl (a : BB) := lb (projy a).
+Definition projyu (a : BB) := ub (projy a).
+
+(** Basic relations of BB. **)
+
+Definition BBeq a b := projx a == projx b /\ projy a == projy b.
+Definition BBsubseteq a b := 
+  Isubseteq (projx a) (projx b) /\ Isubseteq (projy a) (projy b).
+Definition BBoverlap a b :=
+  Ioverlap (projx a) (projx b) /\ Ioverlap (projy a) (projy b).
+Definition BBintersection (a b : BB) : BBoverlap a b -> BB.
+  unfold BBoverlap. destruct a as (ax, ay), b as (bx, _by). simpl.
+  intros (H, H0).
+  exact (Iintersection ax bx H, Iintersection ay _by H0).
+Defined.
+(*
+Definition BBsubset a b :=
+  ((projxl b) <= (projxl a))%nat /\ ((projxu a) < (projxu b))%nat /\
+  ((projyl b) < (projyl a))%nat /\ ((projyu a) < (projyu b))%nat \/
+
+  ((projxl b) < (projxl a))%nat /\ ((projxu a) <= (projxu b))%nat /\
+  ((projyl b) < (projyl a))%nat /\ ((projyu a) < (projyu b))%nat \/
+
+  ((projxl b) < (projxl a))%nat /\ ((projxu a) < (projxu b))%nat /\
+  ((projyl b) <= (projyl a))%nat /\ ((projyu a) < (projyu b))%nat \/
+
+  ((projxl b) < (projxl a))%nat /\ ((projxu a) < (projxu b))%nat /\
+  ((projyl b) < (projyl a))%nat /\ ((projyu a) <= (projyu b))%nat.
+*)
+(*
+Notation Isupset a b := (Isubset b a) (only parsing).
+*)
+Notation Isupseteq a b := (Isubseteq b a) (only parsing).
+
+Infix "==" := BBeq (at level 70, no associativity) : BB_scope.
+
+
+(** * Decidability *)
+
+Theorem BBeq_dec : forall a b, {a == b} + {~ a == b}.
+Proof.
+  unfold BBeq. intros (ax, ay) (bx, _by). simpl.
+  destruct (Ieq_dec ax bx), (Ieq_dec ay _by).
+  - left. split. assumption. assumption.
+  - right. intros (H, H1). apply (n H1).
+  - right. intros (H, H1). apply (n H).
+  - right. intros (H, H1). apply (n H).
+Qed.
+
+
+(** * Properties of basic relations *)
+
+Lemma BBeq_refl : forall a, a == a.
+Proof.
+  unfold BBeq. split.
+  apply Ieq_refl. apply Ieq_refl.
+Qed.
+
+Lemma BBeq_sym : forall a b, a == b -> b == a.
+Proof.
+  unfold BBeq. intros (ax, ay) (bx, _by). simpl.
+  intros (Hax_eq_bx, Hay_eq_by). split.
+  now apply Ieq_sym. now apply Ieq_sym.
+Qed.
+
+Lemma BBeq_sym_iff : forall a b, a == b <-> b == a.
+Proof.
+  split. apply BBeq_sym. apply BBeq_sym.
+Qed.
+
+Lemma BBeq_trans : forall a b c, a == b -> b == c -> a == c.
+Proof.
+  unfold BBeq.
+  intros (ax, ay) (bx, _by) (cx, cy). simpl.
+  intros (Hax_eq_bx, Hay_eq_by) (Hbx_eq_cx, Hby_eq_cy). split.
+  apply (Ieq_trans ax bx cx Hax_eq_bx Hbx_eq_cx).
+  apply (Ieq_trans ay _by cy Hay_eq_by Hby_eq_cy).
+Qed.
+
+(*
+Lemma BBsubset_irrefl : forall a, ~BBsubset a a.
+Proof.
+  unfold BBsubset, projxl, projxu, projyl, projyu.
+  intros (((axl, axu), axp), ((ayl, ayu), ayp)). simpl in axp, ayp. simpl.
+  intros [(H, (H0, (H1, H2))) | [(H, (H0, (H1, H2))) |
+         [(H, (H0, (H1, H2))) | (H, (H0, (H1, H2)))]]].
+  - now apply (Nat.lt_irrefl axu).
+  - now apply (Nat.lt_irrefl ayl).
+  - now apply (Nat.lt_irrefl axu).
+  - now apply (Nat.lt_irrefl axu).
+Qed.
+
+Lemma BBsubset_trans : forall a b c, BBsubset a b -> BBsubset b c -> BBsubset a c.
+Proof.
+  unfold BBsubset, projxl, projxu, projyl, projyu.
+  intros (((axl, axu), axp), ((ayl, ayu), ayp))
+         (((bxl, bxu), bxp), ((byl, byu), byp))
+         (((cxl, cxu), cxp), ((cyl, cyu), cyp)).
+  simpl in axp, ayp, bxp, byp, cxp, cyp. simpl.
+  intros [(H, (H0, (H1, H2))) | [(H, (H0, (H1, H2))) |
+         [(H, (H0, (H1, H2))) | (H, (H0, (H1, H2)))]]]
+         [(H3, (H4, (H5, H6))) | [(H3, (H4, (H5, H6))) |
+         [(H3, (H4, (H5, H6))) | (H3, (H4, (H5, H6)))]]].
+  - left. repeat split.
+    now apply (Nat.le_trans cxl bxl axl).
+    now apply (Nat.lt_trans axu bxu cxu).
+    now apply (Nat.lt_trans cyl byl ayl).
+    now apply (Nat.lt_trans ayu byu cyu).
+  - right; left. repeat split.
+    now apply (Nat.lt_le_trans cxl bxl axl).
+    apply Nat.lt_eq_cases. left. now apply (Nat.lt_le_trans axu bxu cxu).
+    now apply (Nat.lt_trans cyl byl ayl).
+    now apply (Nat.lt_trans ayu byu cyu).
+  - right; right; left. repeat split.
+    now apply (Nat.lt_le_trans cxl bxl axl).
+    now apply (Nat.lt_trans axu bxu cxu).
+    apply Nat.lt_eq_cases. left. now apply (Nat.le_lt_trans cyl byl ayl).
+    now apply (Nat.lt_trans ayu byu cyu).
+  - right; right; right. repeat split.
+    now apply (Nat.lt_le_trans cxl bxl axl).
+    now apply (Nat.lt_trans axu bxu cxu).
+    now apply (Nat.lt_trans cyl byl ayl).
+    apply Nat.lt_eq_cases. left. now apply (Nat.lt_le_trans ayu byu cyu).
+
+  - left. repeat split.
+    apply Nat.lt_eq_cases. left. now apply (Nat.le_lt_trans cxl bxl axl).
+    now apply (Nat.le_lt_trans axu bxu cxu).
+    now apply (Nat.lt_trans cyl byl ayl).
+    now apply (Nat.lt_trans ayu byu cyu).
+  - right; left. repeat split.
+    now apply (Nat.lt_trans cxl bxl axl).
+    now apply (Nat.le_trans axu bxu cxu).
+    now apply (Nat.lt_trans cyl byl ayl).
+    now apply (Nat.lt_trans ayu byu cyu).
+  - right; right; left. repeat split.
+    now apply (Nat.lt_trans cxl bxl axl).
+    now apply (Nat.le_lt_trans axu bxu cxu).
+    apply Nat.lt_eq_cases. left. now apply (Nat.le_lt_trans cyl byl ayl).
+    now apply (Nat.lt_trans ayu byu cyu).
+  - right; right; right. repeat split.
+    now apply (Nat.lt_trans cxl bxl axl).
+    now apply (Nat.le_lt_trans axu bxu cxu).
+    now apply (Nat.lt_trans cyl byl ayl).
+    apply Nat.lt_eq_cases. left. now apply (Nat.lt_le_trans ayu byu cyu).
+
+  - left. repeat split.
+    apply Nat.lt_eq_cases. left. now apply (Nat.le_lt_trans cxl bxl axl).
+    now apply (Nat.lt_trans axu bxu cxu).
+    now apply (Nat.lt_le_trans cyl byl ayl).
+    now apply (Nat.lt_trans ayu byu cyu).
+  - right; left. repeat split.
+    now apply (Nat.lt_trans cxl bxl axl).
+    apply Nat.lt_eq_cases. left. now apply (Nat.lt_le_trans axu bxu cxu).
+    now apply (Nat.lt_le_trans cyl byl ayl).
+    now apply (Nat.lt_trans ayu byu cyu).
+  - right; right; left. repeat split.
+    now apply (Nat.lt_trans cxl bxl axl).
+    now apply (Nat.lt_trans axu bxu cxu).
+    now apply (Nat.le_trans cyl byl ayl).
+    now apply (Nat.lt_trans ayu byu cyu).
+  - right; right; right. repeat split.
+    now apply (Nat.lt_trans cxl bxl axl).
+    now apply (Nat.lt_trans axu bxu cxu).
+    now apply (Nat.lt_le_trans cyl byl ayl).
+    apply Nat.lt_eq_cases. left. now apply (Nat.lt_le_trans ayu byu cyu).
+
+  - left. repeat split.
+    apply Nat.lt_eq_cases. left. now apply (Nat.le_lt_trans cxl bxl axl).
+    now apply (Nat.lt_trans axu bxu cxu).
+    now apply (Nat.lt_trans cyl byl ayl).
+    now apply (Nat.le_lt_trans ayu byu cyu).
+  - right; left. repeat split.
+    now apply (Nat.lt_trans cxl bxl axl).
+    apply Nat.lt_eq_cases. left. now apply (Nat.lt_le_trans axu bxu cxu).
+    now apply (Nat.lt_trans cyl byl ayl).
+    now apply (Nat.le_lt_trans ayu byu cyu).
+  - right; right; left. repeat split.
+    now apply (Nat.lt_trans cxl bxl axl).
+    now apply (Nat.lt_trans axu bxu cxu).
+    apply Nat.lt_eq_cases. left. now apply (Nat.le_lt_trans cyl byl ayl).
+    now apply (Nat.le_lt_trans ayu byu cyu).
+  - right; right; right. repeat split.
+    now apply (Nat.lt_trans cxl bxl axl).
+    now apply (Nat.lt_trans axu bxu cxu).
+    now apply (Nat.lt_trans cyl byl ayl).
+    now apply (Nat.le_trans ayu byu cyu).
+Qed.
+*)
+
+Lemma BBsubseteq_refl : forall a, BBsubseteq a a.
+Proof.
+  unfold BBsubseteq. intros (ax, ay). simpl. split.
+  apply Isubseteq_refl. apply Isubseteq_refl.
+Qed.
+
+Lemma BBsubseteq_antisym : forall a b,
+  BBsubseteq a b -> BBsubseteq b a -> a == b.
+Proof.
+  unfold BBsubseteq, BBeq. intros (ax, ay) (bx, _by). simpl.
+  intros (H, H0) (H1, H2). split.
+  now apply Isubseteq_antisym. now apply Isubseteq_antisym.
+Qed.
+
+Lemma BBsubseteq_trans : forall a b c,
+  BBsubseteq a b -> BBsubseteq b c -> BBsubseteq a c.
+Proof.
+  unfold BBsubseteq. intros (ax, ay) (bx, _by) (cx, cy). simpl.
+  intros (H, H0) (H1, H2). split.
+  apply (Isubseteq_trans ax bx cx H H1). apply (Isubseteq_trans ay _by cy H0 H2).
+Qed.
+
+Lemma BBoverlap_refl : forall a, BBoverlap a a.
+Proof.
+  unfold BBoverlap. intros (ax, ay). simpl. split.
+  apply Ioverlap_refl. apply Ioverlap_refl.
+Qed.
+
+Lemma BBoverlap_sym : forall a b, BBoverlap a b -> BBoverlap b a.
+Proof.
+  unfold BBoverlap. intros (ax, ay) (bx, _by). simpl.
+  intros (H, H1). split. now apply Ioverlap_sym. now apply Ioverlap_sym.
+Qed.
+
+Lemma BBintersection_comm : forall a b (Haob : BBoverlap a b) (Hboa : BBoverlap b a),
+  BBintersection a b Haob == BBintersection b a Hboa.
+Proof.
+  unfold BBintersection, BBeq, BBoverlap, projx. intros (ax, ay) (bx, _by). simpl.
+  intros (H, H0) (H1, H2).  simpl. split.
+  apply (Iintersection_comm ax bx H H1).
+  apply (Iintersection_comm ay _by H0 H2).
+Qed.
+
+(*
 Definition BB : Type := Interval * Interval.
 
 Declare Scope BB_scope.
@@ -121,3 +368,4 @@ Qed.
 
 Definition BBarea (p : BB) : Q :=
   width (projx p) * width (projy p).
+*)
