BBSL/Interval_.v
@@ -1,0 +1,836 @@
+Require Import Arith.
+
+
+(** * Definition of [Interval] *)
+
+(** Intervals are pairs of lower bounds and upper bounds. *)
+
+Definition Interval : Type := { lb_ub : nat * nat | fst lb_ub <= snd lb_ub }.
+
+Declare Scope Interval_scope.
+Open Scope Interval_scope.
+
+Definition lb (i : Interval) : nat := match i with exist _ lb_ub p => fst lb_ub end.
+Definition ub (i : Interval) : nat := match i with exist _ lb_ub jp => snd lb_ub end.
+
+
+(** * Basic relations of ICC (Interval connection calculus) *)
+
+(** disconnected *)
+Definition dcleft i j := ub i < lb j.
+Notation dcright i j := (dcleft j i) (only parsing).
+Notation dc i j := (dcleft i j \/ dcright i j) (only parsing).
+
+Definition ecleft i j := ub i = lb j.
+Notation ecright i j := (ecleft j i) (only parsing).
+(** externally connected *)
+Notation ec i j := (ecleft i j \/ ecright i j) (only parsing).
+
+(** equal *)
+Definition eq i j := lb i = lb j /\ ub i = ub j.
+
+(** partially overlapping *)
+Definition poleft i j := lb i < lb j /\ lb j < ub i /\ ub i < ub j.
+Notation poright i j := (poleft j i) (only parsing).
+Notation po i j := (poleft i j \/ poright i j) (only parsing).
+
+(** tangential proper part *)
+Definition tppleft i j := lb i = lb j /\ ub i < ub j.
+Definition tppright i j := lb j < lb i /\ ub i = ub j.
+Notation tpp i j := (tppleft i j \/ tppright i j) (only parsing).
+
+(** tangential proper part inverse *)
+Notation tppileft i j := (tppleft j i) (only parsing).
+Notation tppiright i j := (tppright j i) (only parsing).
+Notation tppi i j := (tpp j i) (only parsing).
+
+(** non-tangential proper part *)
+Definition ntpp i j := lb j < lb i /\ ub i < ub j.
+
+(** non-tangential proper part inverse *)
+Notation ntppi i j := (ntpp j i) (only parsing).
+
+(** proper part *)
+Definition pp i j := tpp i j \/ ntpp i j.
+
+(** non-proper part *)
+Definition npp i j := pp i j \/ eq i j.
+
+(** overlapping *)
+Definition overlap i j :=
+  ec i j \/ eq i j \/ po i j \/ tpp i j \/ tppi i j \/ ntpp i j \/ ntppi i j.
+
+(** Aliases *)
+Notation lt i j := (dcleft i j) (only parsing).
+Notation subset i j := (pp i j) (only parsing).
+Notation subseteq i j := (npp i j) (only parsing).
+Notation gt i j := (lt j i) (only parsing).
+Notation supset i j := (subset j i) (only parsing).
+Notation supseteq i j := (subseteq j i) (only parsing).
+
+Infix "==" := eq (at level 70, no associativity) : Interval_scope.
+Infix "<" := lt : Interval_scope.
+Notation "x > y" := (lt y x)(only parsing) : Interval_scope.
+Notation "x < y < z" := (x<y/\y<z) : Interval_scope.
+
+
+#[global]
+Hint Unfold dcleft ecleft eq poleft tppleft tppright ntpp pp npp overlap : iarith.
+#[global]
+Hint Extern 5 (?X1 <> ?X2) => intro; discriminate: qarith.
+
+
+(** * Decidability *)
+
+Theorem icc_dec : forall i j,
+  { dcleft i j } + { ecleft i j } + { poleft i j } +
+  { tppiright i j } + { tppleft i j } + { eq i j } + { ntppi i j } +
+  { tppileft i j } + { ntpp i j } + { tppright i j } +
+  { poright i j } + { ecright i j } + { dcright i j }.
+Proof.
+  unfold dcleft, ecleft, poleft, tppright, tppleft, eq, ntpp.
+  destruct i as ((lbi, ubi), p), j as ((lbj, ubj), q). simpl in p, q. simpl.
+  destruct (lt_eq_lt_dec ubi lbj). destruct s.
+  (* dcleft (ubi < lbj) *)
+  - now left; left; left; left; left; left; left; left; left; left; left; left.
+  (* ecleft (ubi = lbj) *)
+  - now left; left; left; left; left; left; left; left; left; left; left; right.
+  - destruct (lt_eq_lt_dec lbi lbj), (lt_eq_lt_dec ubi ubj). destruct s, s0.
+  (* poleft (lbi < lbj < ubi /\ lbj < ubi < ubj) *)
+  -- left; left; left; left; left; left; left; left; left; left; right.
+     repeat split. assumption. assumption. assumption.
+  (* tppiright (lbi < lbj /\ ubi = lbj) *)
+  -- left; left; left; left; left; left; left; left; left; right.
+     split. assumption. now apply eq_sym.
+  (* tppleft (lbi = lbj /\ ubi < ubj) *)
+  -- left; left; left; left; left; left; left; left; right.
+     split. assumption. assumption.
+  (* eq (lbi = lbj /\ ubi = ubj) *)
+  -- left; left; left; left; left; left; left; right.
+     split. assumption. assumption.
+  -- destruct s.
+  (* ntppi (lbi < lbj /\ ubj < ubi) *)
+  --- left; left; left; left; left; left; right.
+      split. assumption. assumption.
+  (* tppileft (lbj = lbi /\ ubj < ubi) *)
+  --- left; left; left; left; left; right.
+      split. now apply eq_sym. assumption.
+  -- destruct s.
+  (* ntpp (lbj < lbi /\ ubi < ubj) *)
+  --- left; left; left; left; right.
+      split. assumption. assumption.
+  (* tppright (lbj < lbi /\ ubi = ubj) *)
+  --- left; left; left; right.
+      split. assumption. assumption.
+  -- destruct (lt_eq_lt_dec lbi ubj). destruct s.
+  (* poright (lbj < lbi < ubj < ubi) *)
+  --- left; left; right.
+      repeat split. assumption. assumption. assumption.
+  (* ecright (lbj = ubi) *)
+  --- left; right. now apply eq_sym.
+  (* dcright (lbi < ubj) *)
+  --- right. assumption.
+Qed.
+
+(*
+Lemma dcleft_not_ecleft : forall i j, dcleft i j -> ~ecleft i j.
+Proof.
+  unfold dcleft, ecleft, not.
+  intros. Nat.order.
+Qed.
+
+Lemma dcleft_not_poleft : forall i j, dcleft i j -> ~poleft i j.
+Proof.
+  unfold dcleft, poleft, not. intros (i, p) (j, q). simpl in p, q. simpl.
+  intros H (H0, (H1, H2)). Nat.order.
+Qed.
+
+Lemma dcleft_not_tppiright : forall i j, dcleft i j -> ~tppiright i j.
+Proof.
+  unfold dcleft, tppiright, not. intros (i, p) (j, q). simpl in p, q. simpl.
+  intros H (H0, H1). Nat.order.
+Qed.
+
+Lemma dcleft_not_tppleft : forall i j, dcleft i j -> ~tppleft i j.
+Proof.
+  unfold dcleft, tppleft, not. intros (i, p) (j, q). simpl in p, q. simpl.
+  intros H (H0, H1). Nat.order.
+Qed.
+
+Lemma dcleft_not_eq : forall i j, dcleft i j -> ~eq i j.
+Proof.
+  unfold dcleft, eq, not. intros (i, p) (j, q). simpl in p, q. simpl.
+  intros H (H0, H1). Nat.order.
+Qed.
+
+Lemma dcleft_not_ntppi : forall i j, dcleft i j -> ~ntppi i j.
+Proof.
+  unfold dcleft, ntppi, not. intros (i, p) (j, q). simpl in p, q. simpl.
+  intros H (H0, H1). Nat.order.
+Qed.
+
+Lemma dcleft_not_tppileft : forall i j, dcleft i j -> ~tppileft i j.
+Proof.
+  unfold dcleft, tppileft, not. intros (i, p) (j, q). simpl in p, q. simpl.
+  intros H (H0, H1). Nat.order.
+Qed.
+
+Lemma dcleft_not_ntpp : forall i j, dcleft i j -> ~ntpp i j.
+Proof.
+  unfold dcleft, ntpp, not. intros (i, p) (j, q). simpl in p, q. simpl.
+  intros H (H0, H1). Nat.order.
+Qed.
+
+Lemma dcleft_not_tppright : forall i j, dcleft i j -> ~tppright i j.
+Proof.
+  unfold dcleft, tppright, not. intros (i, p) (j, q). simpl in p, q. simpl.
+  intros H (H0, H1). Nat.order.
+Qed.
+
+Lemma dcleft_not_poright : forall i j, dcleft i j -> ~poright i j.
+Proof.
+  unfold dcleft, poright, not. intros (i, p) (j, q). simpl in p, q. simpl.
+  intros H (H0, H1). Nat.order.
+Qed.
+
+Lemma dcleft_not_ecright : forall i j, dcleft i j -> ~ecright i j.
+Proof.
+  unfold dcleft, ecright, not. intros (i, p) (j, q). simpl in p, q. simpl.
+  intros H H0. Nat.order.
+Qed.
+
+Lemma dcleft_not_dcright : forall i j, dcleft i j -> ~dcright i j.
+Proof.
+  unfold dcleft, dcright, not. intros (i, p) (j, q). simpl in p, q. simpl.
+  intros H H0. Nat.order.
+Qed.
+*)
+
+
+(** * properties of basic relations *)
+
+Theorem dcleft_irrefl : forall i, ~i < i.
+Proof.
+  auto with iarith.
+  unfold dcleft. intros (i, p). simpl. now apply le_not_lt.
+Qed.
+
+Theorem dcleft_asym : forall i j, i < j -> ~j < i.
+Proof.
+  unfold dcleft. intros (i, p) (j, q). simpl. Nat.order.
+Qed.
+
+Theorem dcleft_trans : forall i j k, i < j -> j < k -> i < k.
+Proof.
+  unfold dcleft. intros (i, p) (j, q) (k, r). simpl. Nat.order.
+Qed.
+
+Lemma dcleft_eq : forall i j k, i < j -> j == k -> i < k.
+Proof.
+  unfold dcleft, eq. intros (i, p) (j, q) (k, r). simpl. intros H (H0, H1). Nat.order.
+Qed.
+
+Lemma eq_dcleft : forall i j k, i == j -> j < k -> i < k.
+Proof.
+  unfold dcleft, eq. intros (i, p) (j, q) (k, r). simpl. intros (H, H0). Nat.order.
+Qed.
+
+Theorem dc_irrefl : forall i, ~dc i i.
+Proof.
+  intros i [H | H]. apply (dcleft_irrefl i H). apply (dcleft_irrefl i H).
+Qed.
+
+Theorem dc_sym : forall i j, dc i j -> dc j i.
+Proof.
+  intros i j [H | H]. now right. now left.
+Qed.
+
+(** ecleft has no theorems *)
+
+Theorem eq_refl : forall i, i == i.
+Proof.
+  unfold eq. split. apply eq_refl. apply eq_refl.
+Qed.
+
+Theorem eq_sym : forall i j, i == j -> j == i.
+Proof.
+  unfold eq. intros i j (H, H0). split.
+  apply (sym_equal H). apply (sym_equal H0).
+Qed.
+
+Lemma eq_sym_iff : forall i j, i == j <-> j == i.
+Proof.
+  split. apply eq_sym. apply eq_sym.
+Qed.
+
+Theorem eq_trans : forall i j k, i == j -> j == k -> i == k.
+Proof.
+  unfold eq. intros i j k (H, H0) (H1, H2). split.
+  apply (eq_trans H H1). apply (eq_trans H0 H2).
+Qed.
+
+Theorem eq_dec : forall i j, {i == j} + {~ i == j}.
+Proof.
+  unfold eq. destruct i as ((lbi, ubi), p), j as ((lbj, ubj), q). simpl in p, q. simpl.
+  destruct (Nat.eq_dec lbi lbj), (Nat.eq_dec ubi ubj).
+  - left. split. assumption. assumption.
+  - right. intros (H, H0). apply (n H0).
+  - right. intros (H, H0). apply (n H).
+  - right. intros (H, H0). apply (n H).
+Qed.
+
+Theorem no_eq_sym i j : ~ i == j -> ~ j == i.
+
+
+Theorem poleft_irrefl : forall i, ~poleft i i.
+Proof.
+  unfold poleft. intros (i, p). simpl. intros (H, H0). apply (lt_irrefl (fst i) H).
+Qed.
+
+Theorem poleft_asym : forall i j, poleft i j -> ~poleft j i.
+Proof.
+  unfold poleft. intros (i, p) (j, q). simpl. intros (H, H0) (H1, H2). Nat.order.
+Qed.
+
+Theorem po_irrefl : forall i, ~po i i.
+Proof.
+  intros i [H | H]. apply (poleft_irrefl i H). apply (poleft_irrefl i H).
+Qed.
+
+Theorem po_sym : forall i j, po i j -> po j i.
+Proof.
+  intros. rewrite or_comm. assumption.
+Qed.
+
+Theorem tppleft_irrefl : forall x, ~tppleft x x.
+Proof.
+  unfold tppleft. intros (i, p). simpl. intros (H, H0). apply (lt_irrefl (snd i) H0).
+Qed.
+
+Theorem tppleft_asym : forall i j, tppleft i j -> ~tppleft j i.
+Proof.
+  unfold tppleft. intros (i, p) (j, q). simpl. intros (H, H0) (H1, H2). Nat.order.
+Qed.
+
+Theorem tppleft_trans : forall i j k, tppleft i j -> tppleft j k -> tppleft i k.
+Proof.
+  unfold tppleft. intros (i, p) (j, q) (k, r). simpl. intros (H, H0) (H1, H2).
+  split. apply (Nat.eq_trans H H1). apply (Nat.lt_trans (snd i) (snd j) (snd k) H0 H2).
+Qed.
+
+Theorem tppright_irrefl : forall i, ~tppright i i.
+Proof.
+  unfold tppright. intros (i, p). simpl. intros (H, H0). apply (lt_irrefl (fst i) H).
+Qed.
+
+Theorem tppright_asym : forall i j, tppright i j -> ~tppright j i.
+  unfold tppright. intros (i, p) (j, q). simpl. intros (H, H0) (H1, H2). Nat.order.
+Qed.
+
+Theorem tppright_trans : forall i j k, tppright i j -> tppright j k -> tppright i k.
+Proof.
+  unfold tppright. intros (i, p) (j, q) (k, r). simpl. intros (H, H0) (H1, H2).
+  split. apply (lt_trans (fst k) (fst j) (fst i) H1 H). apply (Nat.eq_trans H0 H2).
+Qed.
+
+Theorem tpp_irrefl : forall i, ~tpp i i.
+Proof.
+  intros i [H | H]. apply (tppleft_irrefl i H). apply (tppright_irrefl i H).
+Qed.
+
+(*
+Lemma tppleft_not_tppright : forall i j, tppleft i j -> ~tppright i j.
+Proof.
+  unfold tppleft, tppright, not. intros  (i, p) (j, q). simpl in p, q. simpl.
+  intros (H, H0) (H1, H2). Nat.order.
+Qed.
+*)
+
+Theorem tpp_asym : forall i j, tpp i j -> ~tpp j i.
+Proof.
+  unfold tppleft, tppright. intros (i, p) (j, q). simpl in p, q. simpl.
+  intros [(H, H0) | (H, H0)] [(H1, H2) | (H1, H2)].
+  Nat.order. Nat.order. Nat.order. Nat.order.
+Qed.
+
+Theorem ntpp_irrefl : forall i, ~ntpp i i.
+Proof.
+  unfold ntpp. intros i (H, H0). apply (lt_irrefl (lb i) H).
+Qed.
+
+Theorem ntpp_asym : forall i j, ntpp i j -> ~ntpp j i.
+Proof.
+  unfold ntpp. intros i j (H, H0) (H1, H2). Nat.order.
+Qed.
+
+Theorem ntpp_trans : forall i j k, ntpp i j -> ntpp j k -> ntpp i k.
+  unfold ntpp. intros i j k (H, H0) (H1, H2). split. Nat.order. Nat.order.
+Qed.
+
+Theorem pp_irrefl : forall i, ~pp i i.
+Proof.
+  unfold pp. intros i [H | H].
+  apply (tpp_irrefl i H). apply (ntpp_irrefl i H).
+Qed.
+
+Theorem pp_asym : forall i j, pp i j -> ~pp j i.
+Proof.
+  unfold pp, tppleft, tppright, ntpp. intros (i, p) (j, q). simpl in p, q. simpl.
+  intros [[(H, H0) | (H, H0)] | (H, H0)] [[(H1, H2) | (H1, H2)] | (H1, H2)].
+  Nat.order. Nat.order. Nat.order. Nat.order. Nat.order.
+  Nat.order. Nat.order. Nat.order. Nat.order.
+Qed.
+
+Theorem pp_trans : forall i j k, pp i j -> pp j k -> pp i k.
+Proof.
+  unfold pp, tppleft, tppright, ntpp.
+  intros i j k [[(H, H0) | (H, H0)] | (H, H0)] [[(H1, H2) | (H1, H2)] | (H1, H2)].
+  - left. left. split. Nat.order. Nat.order.
+  - right. split. Nat.order. Nat.order.
+  - right. split. Nat.order. Nat.order.
+  - right. split. Nat.order. Nat.order.
+  - left. right. split. Nat.order. Nat.order.
+  - right. split. Nat.order. Nat.order.
+  - right. split. Nat.order. Nat.order.
+  - right. split. Nat.order. Nat.order.
+  - right. split. Nat.order. Nat.order.
+Qed.
+
+Lemma pp_eq : forall i j k, pp i j -> j == k -> pp i k.
+Proof.
+  intros i j k H H0.
+  rewrite H0 in H.
+
+  unfold pp, eq, tppleft, tppright, ntpp.
+  intros i j k [[(H, H0) | (H, H0)] | (H, H0)] (H1, H2).
+  - left. left. split. Nat.order. Nat.order.
+  - left. right. split. Nat.order. Nat.order.
+  - right. split. Nat.order. Nat.order.
+Qed.
+
+Lemma eq_pp : forall i j k, i == j -> pp j k -> pp i k.
+Proof.
+  unfold pp, eq. intros (i, p) (j, q) (k, r). simpl.
+  intros (H, H0) [(H1, H2) | (H1, H2)].
+  - left. split. Nat.order. Nat.order.
+  - right. split. Nat.order. Nat.order.
+Qed.
+
+Theorem npp_refl : forall x, npp x x.
+Proof.
+  unfold npp. intros x. right. now apply eq_sym.
+Qed.
+
+Theorem npp_antisym : forall x y, npp x y -> npp y x -> x == y.
+Proof.
+  unfold npp. intros x y [H | H] [H0 | H0].
+  - now apply pp_asym in H.
+  - now apply eq_sym.
+  - assumption.
+  - assumption.
+Qed.
+
+Theorem npp_trans : forall x y z, npp x y -> npp y z -> npp x z.
+Proof.
+  unfold npp. intros x y z [H | H] [H0 | H0].
+  - left. apply (pp_trans x y z H H0).
+  - left. apply (pp_eq x y z H H0).
+  - left. apply (eq_pp x y z H H0).
+  - right. apply (eq_trans x y z H H0).
+Qed.
+
+Lemma npp_pp_eq : forall i j, npp i j -> pp i j \/ i == j.
+Proof.
+  unfold npp, pp. intros i j [[H | H] | H].
+  - now left; left.
+  - now left; right.
+  - now right.
+Qed.
+
+Notation npp_pp_eq := npp_pp_eq (only parsing).
+
+Theorem overlap_refl : forall i, overlap i i.
+Proof.
+  unfold overlap. intros i. left. apply npp_refl.
+Qed.
+
+Theorem overlap_sym : forall i j, overlap i j -> overlap j i.
+Proof.
+  unfold overlap. intros i j.
+  unfold overlap, pp, eq. intros (i, p) (j, q). simpl. intros [(H, H0)|[(H, H0)|[(H, H0)|[(H, H0)|(H,H0)]]]].
+  - right. left. split. Nat.order. Nat.order.
+  - left. split. Nat.order. Nat.order.
+  - right. right. left. split. Nat.order. Nat.order.
+  - destruct (le_lt_dec (snd i) (snd j)).
+  -- right. right. right. right. split. Nat.order. Nat.order.
+  -- 
+  right. right. right. right. split. Nat.order. Nat.order.
+  - right. right. right. right. split. Nat.order. right. right. right. right. split. Nat.order.
+  - right. left. split. Nat.order. Nat.order.
+  - left. right. split. Nat.order. Nat.order.
+  - right. right. split. Nat.order. Nat.order.
+  - right. right. split. Nat.order. Nat.order.
+  - left. left. split. Nat.order. Nat.order.
+  - left. right. split. Nat.order. Nat.order.
+  - right. left. split. Nat.order. Nat.order.
+  -
+
+
+
+(*
+Lemma porigh_not_rcc : forall i j, poright i j ->
+  ~dcleft i j /\ ~ecleft i j /\ ~poleft i j /\
+  ~tppiright i j /\ ~tppleft i j /\ ~eq i j /\ ~ntppi i j /\
+  ~tppileft i j /\ ~ntpp i j /\ ~tppright i j /\
+  ~ecright i j /\ ~dcright i j.
+Proof.
+  unfold dcleft, ecleft, poleft, tppiright, tppleft, eq, ntppi, tppileft,
+         ntpp, tppright, poright, ecright, dcright, not.
+  intros (i, p) (j, q). simpl. intros ((H, H0), H1). repeat split.
+  - Nat.order.
+  - Nat.order.
+  - intros ((H2, H3), H4). Nat.order.
+  - intros (H2, H3). Nat.order.
+  - intros (H2, H3). Nat.order.
+  - intros (H2, H3). Nat.order.
+  - intros (H2, H3). Nat.order.
+  - intros (H2, H3). Nat.order.
+  - intros (H2, H3). Nat.order.
+  - intros (H2, H3). Nat.order.
+  - Nat.order.
+  - Nat.order.
+Qed.
+
+Lemma ecrigh_not_rcc : forall i j, ecright i j ->
+  ~dcleft i j /\ ~ecleft i j /\ ~poleft i j /\
+  ~tppiright i j /\ ~tppleft i j /\ ~eq i j /\ ~ntppi i j /\
+  ~tppileft i j /\ ~ntpp i j /\ ~tppright i j /\
+  ~poright i j /\ ~dcright i j.
+Proof.
+  unfold dcleft, ecleft, poleft, tppiright, tppleft, eq, ntppi, tppileft,
+         ntpp, tppright, poright, ecright, dcright, not.
+  intros (i, p) (j, q). simpl. intros H. repeat split.
+  - Nat.order.
+  - Nat.order.
+  - intros ((H1, H2), H3). Nat.order.
+  - intros (H1, H2). Nat.order.
+  - intros (H1, H2). Nat.order.
+  - intros (H1, H2). Nat.order.
+  - intros (H1, H2). Nat.order.
+  - intros (H1, H2). Nat.order.
+  - intros (H1, H2). Nat.order.
+  - intros (H1, H2). Nat.order.
+  - intros ((H1, H2), H3). Nat.order.
+  - Nat.order.
+Qed.
+
+Lemma dcrigh_not_rcc : forall i j, dcright i j ->
+  ~dcleft i j /\ ~ecleft i j /\ ~poleft i j /\
+  ~tppiright i j /\ ~tppleft i j /\ ~eq i j /\ ~ntppi i j /\
+  ~tppileft i j /\ ~ntpp i j /\ ~tppright i j /\
+  ~poright i j /\ ~ecright i j.
+Proof.
+  unfold dcleft, ecleft, poleft, tppiright, tppleft, eq, ntppi, tppileft,
+         ntpp, tppright, poright, ecright, dcright, not.
+  intros (i, p) (j, q). simpl. intros H. repeat split.
+  - Nat.order.
+  - Nat.order.
+  - intros ((H1, H2), H3). Nat.order.
+  - intros (H1, H2). Nat.order.
+  - intros (H1, H2). Nat.order.
+  - intros (H1, H2). Nat.order.
+  - intros (H1, H2). Nat.order.
+  - intros (H1, H2). Nat.order.
+  - intros (H1, H2). Nat.order.
+  - intros (H1, H2). Nat.order.
+  - intros ((H1, H2), H3). Nat.order.
+  - Nat.order.
+Qed.
+
+Lemma pp_not_rcc : forall i j, pp i j ->
+  ~dcleft i j /\ ~ecleft i j /\ ~poleft i j /\
+  ~tppiright i j /\ ~eq i j /\ ~ntppi i j /\
+  ~tppileft i j /\
+  ~poright i j /\ ~ecright i j /\ ~dcright i j.
+Proof.
+  unfold pp, tpp. intros i j [[H | H] | H].
+  - apply tppleft_not_rcc in H.
+    destruct H as (H, (H0, (H1, (H2, (H3, (H4, (H5, (H6, (H7, (H8, (H9, H10))))))))))).
+    repeat split.
+    assumption. assumption. assumption. assumption. assumption.
+    assumption. assumption. assumption. assumption. assumption.
+  - apply tppright_not_rcc in H.
+    destruct H as (H, (H0, (H1, (H2, (H3, (H4, (H5, (H6, (H7, (H8, (H9, H10))))))))))).
+    repeat split.
+    assumption. assumption. assumption. assumption. assumption.
+    assumption. assumption. assumption. assumption. assumption.
+  - apply ntpp_not_rcc in H.
+    destruct H as (H, (H0, (H1, (H2, (H3, (H4, (H5, (H6, (H7, (H8, (H9, H10))))))))))).
+    repeat split.
+    assumption. assumption. assumption. assumption. assumption.
+    assumption. assumption. assumption. assumption. assumption.
+Qed.
+
+Lemma npp_not_rcc : forall i j, npp i j ->
+  ~dcleft i j /\ ~ecleft i j /\ ~poleft i j /\
+  ~tppiright i j /\ ~ntppi i j /\
+  ~tppileft i j /\
+  ~poright i j /\ ~ecright i j /\ ~dcright i j.
+Proof.
+  unfold npp. intros i j [H | H].
+  - apply pp_not_rcc in H.
+    destruct H as (H, (H0, (H1, (H2, (H3, (H4, (H5, (H6, (H7, H8))))))))).
+    repeat split.
+    assumption. assumption. assumption. assumption. assumption.
+    assumption. assumption. assumption. assumption.
+  - apply eq_not_rcc in H.
+    destruct H as (H, (H0, (H1, (H2, (H3, (H4, (H5, (H6, (H7, (H8, (H9, H10))))))))))).
+    repeat split.
+    assumption. assumption. assumption. assumption. assumption.
+    assumption. assumption. assumption. assumption.
+Qed.
+
+Lemma overlap_not_lt_gt : forall i j, overlap i j -> ~lt i j /\ ~gt i j.
+Proof.
+  unfold overlap. intros i j [H | [H | [H | [H | [H | [H | [H | [H | [H | [H | H]]]]]]]]]].
+  - apply ecleft_not_rcc in H.
+    destruct H as (H, (H0, (H1, (H2, (H3, (H4, (H5, (H6, (H7, (H8, (H9, H10))))))))))).
+    split. assumption. assumption.
+  - apply ecleft_not_rcc in H.
+    destruct H as (H, (H0, (H1, (H2, (H3, (H4, (H5, (H6, (H7, (H8, (H9, H10))))))))))).
+    split. assumption. assumption.
+  - apply eq_not_rcc in H.
+    destruct H as (H, (H0, (H1, (H2, (H3, (H4, (H5, (H6, (H7, (H8, (H9, H10))))))))))).
+    split. assumption. assumption.
+  - apply poleft_not_rcc in H.
+    destruct H as (H, (H0, (H1, (H2, (H3, (H4, (H5, (H6, (H7, (H8, (H9, H10))))))))))).
+    split. assumption. assumption.
+  - apply poleft_not_rcc in H.
+    destruct H as (H, (H0, (H1, (H2, (H3, (H4, (H5, (H6, (H7, (H8, (H9, H10))))))))))).
+    split. assumption. assumption.
+  - apply tppleft_not_rcc in H.
+    destruct H as (H, (H0, (H1, (H2, (H3, (H4, (H5, (H6, (H7, (H8, (H9, H10))))))))))).
+    split. assumption. assumption.
+  - apply tppleft_not_rcc in H.
+    destruct H as (H, (H0, (H1, (H2, (H3, (H4, (H5, (H6, (H7, (H8, (H9, H10))))))))))).
+    split. assumption. assumption.
+  - apply tppright_not_rcc in H.
+    destruct H as (H, (H0, (H1, (H2, (H3, (H4, (H5, (H6, (H7, (H8, (H9, H10))))))))))).
+    split. assumption. assumption.
+  - apply tppright_not_rcc in H.
+    destruct H as (H, (H0, (H1, (H2, (H3, (H4, (H5, (H6, (H7, (H8, (H9, H10))))))))))).
+    split. assumption. assumption.
+  - apply ntpp_not_rcc in H.
+    destruct H as (H, (H0, (H1, (H2, (H3, (H4, (H5, (H6, (H7, (H8, (H9, H10))))))))))).
+    split. assumption. assumption.
+  - apply ntpp_not_rcc in H.
+    destruct H as (H, (H0, (H1, (H2, (H3, (H4, (H5, (H6, (H7, (H8, (H9, H10))))))))))).
+    split. assumption. assumption.
+Qed.
+
+Lemma dcleft_not_rcc : forall i j, dcleft i j ->
+  ~ecleft i j /\ ~poleft i j /\
+  ~tppiright i j /\ ~tppleft i j /\ ~eq i j /\ ~ntppi i j /\
+  ~tppileft i j /\ ~ntpp i j /\ ~tppright i j /\
+  ~poright i j /\ ~ecright i j /\ ~dcright i j.
+Proof.
+  unfold dcleft, ecleft, poleft, tppiright, tppleft, eq, ntppi, tppileft,
+         ntpp, tppright, poright, ecright, dcright, not.
+  intros (i, p) (j, q). simpl. intros H. repeat split.
+  - Nat.order.
+  - intros ((H0, H1), H2). Nat.order.
+  - intros (H0, H1). Nat.order.
+  - intros (H0, H1). Nat.order.
+  - intros (H0, H1). Nat.order.
+  - intros (H0, H1). Nat.order.
+  - intros (H0, H1). Nat.order.
+  - intros (H0, H1). Nat.order.
+  - intros (H0, H1). Nat.order.
+  - intros (H0, H1). Nat.order.
+  - Nat.order.
+  - Nat.order.
+Qed.
+
+Lemma eq_not_rcc : forall i j, eq i j ->
+  ~dcleft i j /\ ~ecleft i j /\ ~poleft i j /\
+  ~tppiright i j /\ ~tppleft i j /\ ~ntppi i j /\
+  ~tppileft i j /\ ~ntpp i j /\ ~tppright i j /\
+  ~poright i j /\ ~ecright i j /\ ~dcright i j.
+Proof.
+  unfold dcleft, ecleft, poleft, tppiright, tppleft, eq, ntppi, tppileft,
+         ntpp, tppright, poright, ecright, dcright, not.
+  intros (i, p) (j, q). simpl. intros (H, H0). repeat split.
+  - Nat.order.
+  - Nat.order.
+  - intros ((H1, H2), H3). Nat.order.
+  - intros (H1, H2). Nat.order.
+  - intros (H1, H2). Nat.order.
+  - intros (H1, H2). Nat.order.
+  - intros (H1, H2). Nat.order.
+  - intros (H1, H2). Nat.order.
+  - intros (H1, H2). Nat.order.
+  - intros ((H1, H2), H3). Nat.order.
+  - Nat.order.
+  - Nat.order.
+Qed.
+
+Lemma dc_not_rcc : forall i j, dc i j ->
+  ~ecleft i j /\ ~poleft i j /\
+  ~tppiright i j /\ ~tppleft i j /\ ~eq i j /\ ~ntppi i j /\
+  ~tppileft i j /\ ~ntpp i j /\ ~tppright i j /\
+  ~poright i j /\ ~ecright i j.
+Proof.
+  unfold dc. intros i j [H | H].
+  - apply dcleft_not_rcc in H.
+    destruct H as (H, (H0, (H1, (H2, (H3, (H4, (H5, (H6, (H7, (H8, (H9, H10))))))))))).
+    repeat split.
+    assumption. assumption. assumption. assumption. assumption. assumption.
+    assumption. assumption. assumption. assumption. assumption.
+  - apply dcleft_not_rcc in H.
+    destruct H as (H, (H0, (H1, (H2, (H3, (H4, (H5, (H6, (H7, (H8, (H9, H10))))))))))).
+    repeat split.
+    assumption. assumption. assumption. assumption.
+    intros H11. apply (eq_sym i j) in H11.
+    assumption. assumption.
+    assumption. assumption. assumption. assumption. assumption.
+
+Lemma ecleft_not_rcc : forall i j, ecleft i j ->
+  ~dcleft i j /\ ~poleft i j /\
+  ~tppiright i j /\ ~tppleft i j /\ ~eq i j /\ ~ntppi i j /\
+  ~tppileft i j /\ ~ntpp i j /\ ~tppright i j /\
+  ~poright i j /\ ~ecright i j /\ ~dcright i j.
+Proof.
+  unfold dcleft, ecleft, poleft, tppiright, tppleft, eq, ntppi, tppileft,
+         ntpp, tppright, poright, ecright, dcright, not.
+  intros (i, p) (j, q). simpl. intros H. repeat split.
+  - Nat.order.
+  - intros ((H0, H1), H2). Nat.order.
+  - intros (H0, H1). Nat.order.
+  - intros (H0, H1). Nat.order.
+  - intros (H0, H1). Nat.order.
+  - intros (H0, H1). Nat.order.
+  - intros (H0, H1). Nat.order.
+  - intros (H0, H1). Nat.order.
+  - intros (H0, H1). Nat.order.
+  - intros (H0, H1). Nat.order.
+  - Nat.order.
+  - Nat.order.
+Qed.
+
+Lemma poleft_not_rcc : forall i j, poleft i j ->
+  ~dcleft i j /\ ~ecleft i j /\
+  ~tppiright i j /\ ~tppleft i j /\ ~eq i j /\ ~ntppi i j /\
+  ~tppileft i j /\ ~ntpp i j /\ ~tppright i j /\
+  ~poright i j /\ ~ecright i j /\ ~dcright i j.
+Proof.
+  unfold dcleft, ecleft, poleft, tppiright, tppleft, eq, ntppi, tppileft,
+         ntpp, tppright, poright, ecright, dcright, not.
+  intros (i, p) (j, q). simpl. intros ((H, H0), H1). repeat split.
+  - Nat.order.
+  - Nat.order.
+  - intros (H2, H3). Nat.order.
+  - intros (H2, H3). Nat.order.
+  - intros (H2, H3). Nat.order.
+  - intros (H2, H3). Nat.order.
+  - intros (H2, H3). Nat.order.
+  - intros (H2, H3). Nat.order.
+  - intros (H2, H3). Nat.order.
+  - intros ((H2, H3), H4). Nat.order.
+  - Nat.order.
+  - Nat.order.
+Qed.
+
+Lemma tppleft_not_rcc : forall i j, tppleft i j ->
+  ~dcleft i j /\ ~ecleft i j /\ ~poleft i j /\
+  ~tppiright i j /\ ~eq i j /\ ~ntppi i j /\
+  ~tppileft i j /\ ~ntpp i j /\ ~tppright i j /\
+  ~poright i j /\ ~ecright i j /\ ~dcright i j.
+Proof.
+  unfold dcleft, ecleft, poleft, tppiright, tppleft, eq, ntppi, tppileft,
+         ntpp, tppright, poright, ecright, dcright, not.
+  intros (i, p) (j, q). simpl. intros (H, H0). repeat split.
+  - Nat.order.
+  - Nat.order.
+  - intros ((H1, H2), H3). Nat.order.
+  - intros (H1, H2). Nat.order.
+  - intros (H1, H2). Nat.order.
+  - intros (H1, H2). Nat.order.
+  - intros (H1, H2). Nat.order.
+  - intros (H1, H2). Nat.order.
+  - intros (H1, H2). Nat.order.
+  - intros ((H1, H2), H3). Nat.order.
+  - Nat.order.
+  - Nat.order.
+Qed.
+
+Lemma tppright_not_rcc : forall i j, tppright i j ->
+  ~dcleft i j /\ ~ecleft i j /\ ~poleft i j /\
+  ~tppiright i j /\ ~tppleft i j /\ ~eq i j /\ ~ntppi i j /\
+  ~tppileft i j /\ ~ntpp i j /\
+  ~poright i j /\ ~ecright i j /\ ~dcright i j.
+Proof.
+  unfold dcleft, ecleft, poleft, tppiright, tppleft, eq, ntppi, tppileft,
+         ntpp, tppright, poright, ecright, dcright, not.
+  intros (i, p) (j, q). simpl. intros (H, H0). repeat split.
+  - Nat.order.
+  - Nat.order.
+  - intros ((H1, H2), H3). Nat.order.
+  - intros (H1, H2). Nat.order.
+  - intros (H1, H2). Nat.order.
+  - intros (H1, H2). Nat.order.
+  - intros (H1, H2). Nat.order.
+  - intros (H1, H2). Nat.order.
+  - intros (H1, H2). Nat.order.
+  - intros ((H1, H2), H3). Nat.order.
+  - Nat.order.
+  - Nat.order.
+Qed.
+
+Lemma ntpp_not_rcc : forall i j, ntpp i j ->
+  ~dcleft i j /\ ~ecleft i j /\ ~poleft i j /\
+  ~tppiright i j /\ ~tppleft i j /\ ~eq i j /\ ~ntppi i j /\
+  ~tppileft i j /\ ~tppright i j /\
+  ~poright i j /\ ~ecright i j /\ ~dcright i j.
+Proof.
+  unfold dcleft, ecleft, poleft, tppiright, tppleft, eq, ntppi, tppileft,
+         ntpp, tppright, poright, ecright, dcright, not.
+  intros (i, p) (j, q). simpl. intros (H, H0). repeat split.
+  - Nat.order.
+  - Nat.order.
+  - intros ((H1, H2), H3). Nat.order.
+  - intros (H1, H2). Nat.order.
+  - intros (H1, H2). Nat.order.
+  - intros (H1, H2). Nat.order.
+  - intros (H1, H2). Nat.order.
+  - intros (H1, H2). Nat.order.
+  - intros (H1, H2). Nat.order.
+  - intros ((H1, H2), H3). Nat.order.
+  - Nat.order.
+  - Nat.order.
+Qed.
+*)
+
+(*
+Definition lt_irrefl := dcleft_irrefl.
+Definition lt_asym := dcleft_asym.
+Definition lt_trans := dcleft_trans.
+Definition lt_eq := dcleft_eq.
+Definition eq_lt := eq_dcleft.
+*)
+
+Lemma lt_overlap_lt_dec : forall i j, { i < j } + { overlap i j } + { j < i }.
+
+Lemma intersection_comm : forall i j (H : overlap i j), intersection i j H == intersection j i H.
+
+(* operators *)
+
+Definition intersection (i j : Interval) : overlap i j -> Interval.
+  (*destruct i as (i, p), j as (j, q). simpl. intros H. simpl in H.*)
+  intros H. destruct H.
+  assert (max (fst i) (fst j) < min (snd i) (snd j))%nat.
+  rewrite Nat.max_lub_lt_iff, Nat.min_glb_lt_iff, Nat.min_glb_lt_iff.
+  destruct H as [H | H]. (*destruct H. [(H, H0)|(H, H0)].*)
+  repeat split. Nat.order. Nat.order. Nat.order. Nat.order.
+  repeat split. Nat.order. Nat.order. Nat.order. Nat.order.
+  exact (exist _ (max (fst i) (fst j), min (snd i) (snd j)) H0).
+Qed.
