Examples/comparison_with_binary_topological_relationships.v
@@ -1,0 +1,126 @@
+Require Import List QArith String.
+Require Import BBSL.BBSL.
+Import ListNotations.
+
+Local Open Scope string_scope.
+Local Open Scope BBSL_scope.
+
+
+Definition example_contains : Spec :=
+  ( CND_None
+  , [ ( "A contains B"
+      , [ DEF_BB "A" (EXP_BBvar "Aを返す関数")
+        ; DEF_BB "B" (EXP_BBvar "Bを返す関数")
+        ]
+      , EXP_and
+         (EXP_BBsupseteq (EXP_BBvar "A") (EXP_BBvar "B"))
+         (EXP_not (EXP_or
+           (EXP_Qeq (EXP_projxl (EXP_BBvar "A")) (EXP_projxl (EXP_BBvar "B")))
+           (EXP_or
+             (EXP_Qeq (EXP_projxu (EXP_BBvar "A")) (EXP_projxu (EXP_BBvar "B")))
+             (EXP_or
+               (EXP_Qeq (EXP_projyl (EXP_BBvar "A")) (EXP_projyl (EXP_BBvar "B")))
+               (EXP_Qeq (EXP_projyu (EXP_BBvar "A")) (EXP_projyu (EXP_BBvar "B")))))))
+      )
+    ; ( "A covers B"
+      , [ DEF_BB "A" (EXP_BBvar "Aを返す関数")
+        ; DEF_BB "B" (EXP_BBvar "Bを返す関数")
+        ]
+      , EXP_and
+         (EXP_BBsupseteq (EXP_BBvar "A") (EXP_BBvar "B"))
+         (EXP_or
+           (EXP_Qeq (EXP_projxl (EXP_BBvar "A")) (EXP_projxl (EXP_BBvar "B")))
+           (EXP_or
+             (EXP_Qeq (EXP_projxu (EXP_BBvar "A")) (EXP_projxu (EXP_BBvar "B")))
+             (EXP_or
+               (EXP_Qeq (EXP_projyu (EXP_BBvar "A")) (EXP_projyl (EXP_BBvar "B")))
+               (EXP_Qeq (EXP_projyl (EXP_BBvar "A")) (EXP_projyu (EXP_BBvar "B"))))))
+      )
+    ; ( "A touch B"
+      , [ DEF_BB "A" (EXP_BBvar "Aを返す関数")
+        ; DEF_BB "B" (EXP_BBvar "Bを返す関数")
+        ]
+      , EXP_and
+          (EXP_Qeq
+            (EXP_RAT
+              (EXP_SBBintersection (EXP_makeSBB [ EXP_BBvar "A" ]) (EXP_makeSBB [ EXP_BBvar "B" ]))
+              (EXP_SBBunion (EXP_makeSBB [ EXP_BBvar "A" ]) (EXP_makeSBB [ EXP_BBvar "B" ])))
+            (EXP_Q 0))
+          (EXP_or
+            (EXP_Qeq (EXP_projxl (EXP_BBvar "A")) (EXP_projxl (EXP_BBvar "B")))
+            (EXP_or
+              (EXP_Qeq (EXP_projxu (EXP_BBvar "A")) (EXP_projxu (EXP_BBvar "B")))
+              (EXP_or
+              (EXP_Qeq (EXP_projyl (EXP_BBvar "A")) (EXP_projyl (EXP_BBvar "B")))
+              (EXP_Qeq (EXP_projyu (EXP_BBvar "A")) (EXP_projyu (EXP_BBvar "B"))))))
+      )
+    ; ( "A overlapbdyintersect B"
+      , [ DEF_BB "A" (EXP_BBvar "Aを返す関数")
+        ; DEF_BB "B" (EXP_BBvar "Bを返す関数")
+        ]
+      , EXP_not (EXP_and
+          (EXP_Qeq
+            (EXP_RAT
+              (EXP_SBBintersection (EXP_makeSBB [ EXP_BBvar "A" ]) (EXP_makeSBB [ EXP_BBvar "B" ]))
+              (EXP_makeSBB [ EXP_BBvar "B" ]))
+            (EXP_Q 1))
+          (EXP_Qeq
+            (EXP_RAT
+              (EXP_SBBintersection (EXP_makeSBB [ EXP_BBvar "A" ]) (EXP_makeSBB [ EXP_BBvar "B" ]))
+              (EXP_makeSBB [ EXP_BBvar "B" ]))
+            (EXP_Q 0)))
+      )
+    ; ( "A equal B"
+      , [ DEF_BB "A" (EXP_BBvar "Aを返す関数")
+        ; DEF_BB "B" (EXP_BBvar "Bを返す関数")
+        ]
+      , EXP_BBeq (EXP_BBvar "A") (EXP_BBvar "B")
+      )
+    ; ( "A disjoint B"
+      , [ DEF_BB "A" (EXP_BBvar "Aを返す関数")
+        ; DEF_BB "B" (EXP_BBvar "Bを返す関数")
+        ]
+      , EXP_not (EXP_BBoverlap (EXP_BBvar "A") (EXP_BBvar "B"))
+      )
+    ; ( "A overlapbdydisjoint B"
+      , [ DEF_BB "A" (EXP_BBvar "Aを返す関数")
+        ; DEF_BB "B" (EXP_BBvar "Bを返す関数")
+        ]
+      , EXP_or
+          (EXP_and
+            (EXP_Qeq (EXP_width (EXP_projy (EXP_BBvar "B"))) (EXP_Q 0))
+            (EXP_or
+              (EXP_and
+                (EXP_Iin (EXP_projxl (EXP_BBvar "A")) (EXP_projx (EXP_BBvar "B")))
+                (EXP_Iin (EXP_projxu (EXP_BBvar "A")) (EXP_projx (EXP_BBvar "B"))))
+              (EXP_and
+                (EXP_Iin (EXP_projxu (EXP_BBvar "A")) (EXP_projx (EXP_BBvar "B")))
+                (EXP_not (EXP_Iin (EXP_projxl (EXP_BBvar "A")) (EXP_projx (EXP_BBvar "B")))))))
+          (EXP_and
+            (EXP_Qeq (EXP_width (EXP_projx (EXP_BBvar "B"))) (EXP_Q 0))
+            (EXP_or
+              (EXP_and
+                (EXP_Iin (EXP_projyl (EXP_BBvar "A")) (EXP_projy (EXP_BBvar "B")))
+                (EXP_Iin (EXP_projyu (EXP_BBvar "A")) (EXP_projy (EXP_BBvar "B"))))
+              (EXP_and
+                (EXP_Iin (EXP_projyu (EXP_BBvar "A")) (EXP_projy (EXP_BBvar "B")))
+                (EXP_not (EXP_Iin (EXP_projyl (EXP_BBvar "A")) (EXP_projy (EXP_BBvar "B")))))))
+      )
+    ; ( "A on B"
+      , [ DEF_BB "A" (EXP_BBvar "Aを返す関数")
+        ; DEF_BB "B" (EXP_BBvar "Bを返す関数")
+        ]
+      , EXP_or
+          (EXP_and
+            (EXP_Qeq (EXP_width (EXP_projy (EXP_BBvar "B"))) (EXP_Q 0))
+            (EXP_or
+              (EXP_Iinrev (EXP_projy (EXP_BBvar "B")) (EXP_projyu (EXP_BBvar "A")))
+              (EXP_Iinrev (EXP_projy (EXP_BBvar "B")) (EXP_projyl (EXP_BBvar "A")))))
+          (EXP_and
+            (EXP_Qeq (EXP_width (EXP_projx (EXP_BBvar "B"))) (EXP_Q 0))
+            (EXP_or
+              (EXP_Iinrev (EXP_projx (EXP_BBvar "B")) (EXP_projxu (EXP_BBvar "A")))
+              (EXP_Iinrev (EXP_projx (EXP_BBvar "B")) (EXP_projxl (EXP_BBvar "A")))))
+      )
+    ]
+  ).
