Examples/confluence.v
@@ -1,0 +1,108 @@
+Require Import List String.
+Require Import BBSL.BBSL.
+Import ListNotations.
+
+Local Open Scope string_scope.
+Local Open Scope BBSL_scope.
+
+
+Definition example_confluence : Spec := 
+  ( CND_None
+  , [ ( "シーン１"
+      , [ DEF_I "合流領域" (EXP_Ivar "合流領域")
+        ; DEF_SBB "他車集合" (EXP_SBBvar "他車集合")
+        ]
+      , EXP_forall "x" (EXP_SBBvar "他車集合")
+          (EXP_not (EXP_Ieq (EXP_projy (EXP_BBvar "x")) (EXP_Ivar "合流領域")))
+      )
+    ; ( "シーン２"
+      , [ DEF_I "合流領域" (EXP_Ivar "合流領域")
+        ; DEF_SBB "他車集合" (EXP_SBBvar "他車集合")
+        ]
+      , EXP_exists "x" (EXP_SBBvar "他車集合")
+          (EXP_and
+            (EXP_Qeq (EXP_projyl (EXP_BBvar "x")) (EXP_proju (EXP_Ivar "合流領域")))
+            (EXP_forall "y" (EXP_SBBvar "他車集合")
+              (EXP_or (EXP_not (EXP_Ieq (EXP_projy (EXP_BBvar "y")) (EXP_Ivar "合流領域")))
+                      (EXP_BBeq (EXP_BBvar "x") (EXP_BBvar "y")))))
+      )
+    ; ( "シーン３"
+      , [ DEF_I "合流領域" (EXP_Ivar "合流領域")
+        ; DEF_SBB "他車集合" (EXP_SBBvar "他車集合")
+        ]
+      , EXP_exists "x" (EXP_SBBvar "他車集合")
+         (EXP_and
+           (EXP_Qeq (EXP_projyl (EXP_BBvar "x")) (EXP_proju (EXP_Ivar "合流領域")))
+           (EXP_and
+             (EXP_exists "y" (EXP_SBBvar "他車集合")
+               (EXP_and
+                 (EXP_Qeq (EXP_projyu (EXP_BBvar "y")) (EXP_projl (EXP_Ivar "合流領域")))
+                 (EXP_not (EXP_BBeq (EXP_BBvar "x") (EXP_BBvar "y")))))
+             (EXP_forall "z" (EXP_SBBvar "他車領域")
+                   (EXP_not (EXP_Isupseteq (EXP_Ivar "合流領域") (EXP_projy (EXP_BBvar "z")))))))
+      )
+    ; ( "シーン４"
+      , [ DEF_I "合流領域" (EXP_Ivar "合流領域")
+        ; DEF_SBB "他車集合" (EXP_SBBvar "他車集合")
+        ]
+      , EXP_exists "z" (EXP_SBBvar "他車集合")
+          (EXP_Isupseteq (EXP_Ivar "合流領域") (EXP_projy (EXP_BBvar "z")))
+      )
+    ]
+  ).
+
+(*
+Proposition comprehensiveness_of_example_confluence :
+  forall (confluent_region : Interval) (set_of_cars : SetBB),
+    let evaluated := 
+      Cspec
+        example_confluence
+        (add "合流領域" (Vi confluent_region) (add "他車集合" (Vsbb set_of_cars) (empty Value)))
+    in 
+    Inempty confluent_region ->
+       match option_map (fun ev => List.fold_left or (List.map snd ev) False) evaluated with
+       | Some b => b
+       | _ => False
+       end.
+Proof.
+  simpl.
+  intros confluent_region set_of_cars. destruct confluent_region as (region_l, region_u).
+  destruct set_of_cars as [|car].
+  -- simpl. rewrite (and_l True True).
+     rewrite (or_truer (((False \/ True /\ False) \/ True /\ False) \/ True /\ False)).
+     trivial.
+     trivial.
+  -- destruct car as (car_x, car_y).
+     destruct car_x as (car_xl, car_xu).
+     destruct car_y as (car_yl, car_yu).
+     simpl. unfold Inempty. unfold Ieq. unfold Isubseteq. simpl.
+
+     destruct (Qlt_le_dec )
+
+  destruct dec as (dec_x, dec_y). destruct front_bb as (f_x, f_y).
+  destruct dec_x as (dec_xl, dec_xu). destruct dec_y as (dec_yl, dec_yu).
+  destruct f_x as (f_xl, f_xu). destruct f_y as (f_yl, f_yu).
+  simpl. simpl in H. destruct H. destruct H. destruct H0. destruct H0.
+  rewrite (Q.min_lt_iff f_yu dec_yu (Qmax f_yl dec_yl)).
+  rewrite (Q.max_lt_iff f_yl dec_yl dec_yu).
+  rewrite (Q.max_lt_iff f_yl dec_yl f_yu).
+  destruct (Qlt_le_dec dec_yu f_yl).
+  - left. left. right. apply (conj H2 q).
+  - destruct (Qlt_le_dec f_yu dec_yl).
+  -- left. right. apply (conj H2 q0).
+  -- right. split. assumption. intros. destruct H4. destruct H4.
+  --- apply (Qle_lteq f_yl f_yu) in H1. destruct H1.
+  ---- apply (Qlt_asym f_yl f_yu (conj H1 H4)).
+  ---- rewrite H1 in H4. apply (Qlt_irrefl f_yu H4).
+  --- apply (Qle_lteq dec_yl f_yu) in q0. destruct q0.
+  ---- apply (Qlt_asym dec_yl f_yu (conj H5 H4)).
+  ---- rewrite H5 in H4. apply (Qlt_irrefl f_yu H4).
+  --- destruct H4.
+  ---- apply (Qle_lteq f_yl dec_yu) in q. destruct q.
+  ----- apply (Qlt_asym f_yl dec_yu (conj H5 H4)).
+  ----- rewrite H5 in H4. apply (Qlt_irrefl dec_yu H4).
+  ---- apply (Qle_lteq dec_yl dec_yu) in H3. destruct H3.
+  ----- apply (Qlt_asym dec_yl dec_yu (conj H3 H4)).
+  ----- rewrite H3 in H4. apply (Qlt_irrefl dec_yu H4).
+Qed.
+*)
