Examples/debris_static_in_lane.v
@@ -1,0 +1,76 @@
+Require Import List String.
+Require Import BBSL.BBSL.
+Import ListNotations.
+
+Local Open Scope string_scope.
+Local Open Scope BBSL_scope.
+
+
+Definition example_debris_static_in_lane : Spec :=
+  ( CND (EXP_Bvar "静的障害物がある")
+  , [ ( "減速"
+      , [ DEF_SBB "障害物集合" (EXP_SBBvar "障害物集合")
+        ; DEF_SBB "進行区間集合" (EXP_SBBvar "進行区間集合")
+        ; DEF_BB "減速区間" (EXP_BBvar "減速区間")
+        ]
+      , EXP_exists "x" (EXP_SBBvar "障害物集合")
+          (EXP_exists "y" (EXP_SBBvar "進行区間集合")
+            (EXP_and
+              (EXP_Ioverlap (EXP_projx (EXP_BBvar "x")) (EXP_projx (EXP_BBvar "y")))
+              (EXP_and
+                (EXP_Ioverlap (EXP_projy (EXP_BBvar "x")) (EXP_projy (EXP_BBvar "y")))
+                (EXP_Ioverlap (EXP_projy (EXP_BBvar "x")) (EXP_projy (EXP_BBvar "減速区間"))))))
+      )
+    ; ( "停止"
+      , [ DEF_SBB "障害物集合" (EXP_SBBvar "障害物集合")
+        ; DEF_SBB "進行区間集合" (EXP_SBBvar "進行区間集合")
+        ; DEF_BB "減速区間" (EXP_BBvar "減速区間")
+        ]
+      , EXP_exists "x" (EXP_SBBvar "障害物集合")
+          (EXP_exists "y" (EXP_SBBvar "進行区間集合")
+            (EXP_and
+              (EXP_Ioverlap (EXP_projx (EXP_BBvar "x")) (EXP_projx (EXP_BBvar "y")))
+              (EXP_and
+                (EXP_Ioverlap (EXP_projy (EXP_BBvar "x")) (EXP_projy (EXP_BBvar "y")))
+                (EXP_Ilt (EXP_projy (EXP_BBvar "x")) (EXP_projy (EXP_BBvar "減速区間"))))))
+      )
+    ; ( "レスポンスなし"
+      , [ DEF_SBB "障害物集合" (EXP_SBBvar "障害物集合")
+        ; DEF_SBB "進行区間集合" (EXP_SBBvar "進行区間集合")
+        ; DEF_BB "減速区間" (EXP_BBvar "減速区間")
+        ]
+      , EXP_exists "x" (EXP_SBBvar "障害物集合")
+          (EXP_exists "y" (EXP_SBBvar "進行区間集合")
+            (EXP_and
+              (EXP_Ioverlap (EXP_projx (EXP_BBvar "x")) (EXP_projx (EXP_BBvar "y")))
+              (EXP_and
+                (EXP_Ioverlap (EXP_projy (EXP_BBvar "x")) (EXP_projy (EXP_BBvar "y")))
+                (EXP_Igt (EXP_projy (EXP_BBvar "x")) (EXP_projy (EXP_BBvar "減速区間"))))))
+      )
+    ]
+  ).
+
+(**
+Proposition comprehensiveness_of_example_debris_static_in_lane :
+  forall (exists_debris : Prop) (debrises : SetBB) (lane_bbs : SetBB) (dec : BB),
+    let evaluated :=
+      Cspec
+        example_debris_static_in_lane
+        (add "減速区間" (Vbb dec) (add "進行区間集合" (Vsbb lane_bbs) (add "障害物集合" (Vsbb debrises) (add "静的障害物がある" (Vb exists_debris) (empty Value)))))
+    in
+    BBnempty dec /\ exists_debris ->
+      match option_map (fun ev => List.fold_left or (List.map snd ev) False) evaluated with
+      | Some b => b
+      | _ => False
+      end.
+Proof.
+  simpl. unfold BBnempty. unfold Inempty. unfold Igt. unfold Ilt.
+  unfold Ioverlap. unfold Iempty. unfold Iintersection. unfold not.
+  intros. destruct dec as (dec_x, dec_y). 
+  destruct dec_x as (dec_xl, dec_xu). destruct dec_y as (dec_yl, dec_yu).
+  simpl. simpl in H. destruct H. destruct H. destruct H0. destruct H0.
+  rewrite (Q.min_lt_iff f_yu dec_yu (Qmax f_yl dec_yl)).
+  rewrite (Q.max_lt_iff f_yl dec_yl dec_yu).
+  rewrite (Q.max_lt_iff f_yl dec_yl f_yu).
+  destruct (Qlt_le_dec dec_yu f_yl).
+*)
