Examples/vehicle_cutting_in.v
@@ -1,0 +1,56 @@
+Require Import List String.
+Require Import BBSL.BBSL.
+Import ListNotations.
+
+Local Open Scope string_scope.
+Local Open Scope BBSL_scope.
+
+
+Definition example_vehicle_cutting_in : Spec :=
+  ( CND (EXP_and (EXP_Bvar "前方車両がある") (EXP_Bvar "他車両がある"))
+  , [ ( "停止"
+      , [ DEF_BB "割り込み車両" (EXP_BBvar "割り込み車両")
+        ; DEF_SBB "自車線区間集合" (EXP_SBBvar "自車線区間集合")
+        ; DEF_BB "減速区間" (EXP_BBvar "減速区間")
+        ]
+      , EXP_exists "x" (EXP_SBBvar "自車線区間集合")
+          (EXP_and
+            (EXP_Ioverlap (EXP_projx (EXP_BBvar "割り込み車両")) (EXP_projx (EXP_BBvar "x")))
+            (EXP_Ioverlap (EXP_projy (EXP_BBvar "割り込み車両")) (EXP_projy (EXP_BBvar "減速区間"))))
+      )
+    ; ( "減速"
+      , [ DEF_BB "割り込み車両" (EXP_BBvar "割り込み車両")
+        ; DEF_SBB "自車線区間集合" (EXP_SBBvar "自車線区間集合")
+        ; DEF_BB "減速区間" (EXP_BBvar "減速区間")
+        ]
+      , EXP_and
+          (EXP_forall "x" (EXP_SBBvar "自車線区間集合")
+            (EXP_and
+              (EXP_not (EXP_Ioverlap (EXP_projx (EXP_BBvar "割り込み車両")) (EXP_projx (EXP_BBvar "x"))))
+              (EXP_Ilt (EXP_projy (EXP_BBvar "割り込み車両")) (EXP_projy (EXP_BBvar "減速区間")))))
+          (EXP_exists "x" (EXP_SBBvar "自車線区間")
+            (EXP_and
+              (EXP_Ioverlap (EXP_projx (EXP_BBvar "割り込み車両")) (EXP_projx (EXP_BBvar "x")))
+              (EXP_Ioverlap (EXP_projy (EXP_BBvar "割り込み車両")) (EXP_projy (EXP_BBvar "減速区間")))))
+      )
+    ; ( "前方車両に従う"
+      , [ DEF_BB "割り込み車両" (EXP_BBvar "割り込み車両")
+        ; DEF_BB "前方車両" (EXP_BBvar "前方車両")
+        ]
+      , EXP_Qlt (EXP_projyl (EXP_BBvar "前方車両")) (EXP_projyl (EXP_BBvar "割り込み車両"))
+      )
+    ; ( "割り込み車両に前方を譲る"
+      , [ DEF_BB "割り込み車両" (EXP_BBvar "割り込み車両")
+        ; DEF_SBB "自車線区間集合" (EXP_SBBvar "自車線区間集合")
+        ; DEF_BB "減速区間" (EXP_BBvar "減速区間")
+        ]
+      , EXP_forall "x" (EXP_SBBvar "自車線区間集合")
+          (EXP_not
+            (EXP_and
+              (EXP_Ioverlap (EXP_projx (EXP_BBvar "割り込み車両")) (EXP_projx (EXP_BBvar "x")))
+              (EXP_or
+                (EXP_Ilt (EXP_projy (EXP_BBvar "割り込み車両")) (EXP_projy (EXP_BBvar "減速区間")))
+                (EXP_Ioverlap (EXP_projy (EXP_BBvar "割り込み車両")) (EXP_projy (EXP_BBvar "減速区間"))))))
+      )
+    ]
+  ).
